src/HOL/Imperative_HOL/Relational.thy
@@ -2,81 +2,38 @@ theory Relational
 imports Array Ref
 begin
 
-section{* Definition of the Relational framework *}
+lemma crel_assert_eq: "(\<And>h h' r. crel f h h' r \<Longrightarrow> P r) \<Longrightarrow> f \<guillemotright>= assert P = f"
+unfolding crel_def bind_def Let_def assert_def
+  raise_def return_def prod_case_beta
+apply (cases f)
+apply simp
+apply (simp add: expand_fun_eq split_def)
+apply (auto split: option.split)
+done
 
-text {* The crel predicate states that when a computation c runs with the heap h
-  will result in return value r and a heap h' (if no exception occurs). *}  
+lemma crel_option_caseI:
+  assumes "\<And>y. x = Some y \<Longrightarrow> crel (s y) h h' r"
+  assumes "x = None \<Longrightarrow> crel n h h' r"
+  shows "crel (case x of None \<Rightarrow> n | Some y \<Rightarrow> s y) h h' r"
+using assms
+by (auto split: option.split)
 
-definition crel :: "'a Heap \<Rightarrow> heap \<Rightarrow> heap \<Rightarrow> 'a \<Rightarrow> bool"
-where
-  crel_def': "crel c h h' r \<longleftrightarrow> Heap_Monad.execute c h = Some (r, h')"
+lemma crelI2:
+  assumes "\<exists>h' rs'. crel f h h' rs' \<and> (\<exists>h'' rs. crel (g rs') h' h'' rs)"
+  shows "\<exists>h'' rs. crel (f\<guillemotright>= g) h h'' rs"
+  oops
 
-lemma crel_def: -- FIXME
-  "crel c h h' r \<longleftrightarrow> Some (r, h') = Heap_Monad.execute c h"
-  unfolding crel_def' by auto
-
-lemma crel_deterministic: "\<lbrakk> crel f h h' a; crel f h h'' b \<rbrakk> \<Longrightarrow> (a = b) \<and> (h' = h'')"
-unfolding crel_def' by auto
-
-section {* Elimination rules *}
-
-text {* For all commands, we define simple elimination rules. *}
-(* FIXME: consumes 1 necessary ?? *)
-
-lemma crel_tap:
-  assumes "crel (Heap_Monad.tap f) h h' r"
-  obtains "h' = h" "r = f h"
-  using assms by (simp add: crel_def)
-
-lemma crel_heap:
-  assumes "crel (Heap_Monad.heap f) h h' r"
-  obtains "h' = snd (f h)" "r = fst (f h)"
-  using assms by (cases "f h") (simp add: crel_def)
-
-lemma crel_guard:
-  assumes "crel (Heap_Monad.guard P f) h h' r"
-  obtains "h' = snd (f h)" "r = fst (f h)" "P h"
-  using assms by (cases "f h", cases "P h") (simp_all add: crel_def execute_simps)
-
-
-subsection {* Elimination rules for basic monadic commands *}
-
-lemma crelE[consumes 1]:
-  assumes "crel (f >>= g) h h'' r'"
-  obtains h' r where "crel f h h' r" "crel (g r) h' h'' r'"
-  using assms by (auto simp add: crel_def bind_def split: option.split_asm)
-
-lemma crelE'[consumes 1]:
-  assumes "crel (f >> g) h h'' r'"
-  obtains h' r where "crel f h h' r" "crel g h' h'' r'"
-  using assms
-  by (elim crelE) auto
-
-lemma crel_return[consumes 1]:
-  assumes "crel (return x) h h' r"
-  obtains "r = x" "h = h'"
-  using assms
-  unfolding crel_def return_def by simp
-
-lemma crel_raise[consumes 1]:
-  assumes "crel (raise x) h h' r"
-  obtains "False"
-  using assms
-  unfolding crel_def raise_def by simp
-
-lemma crel_if:
-  assumes "crel (if c then t else e) h h' r"
-  obtains "c" "crel t h h' r"
-        | "\<not>c" "crel e h h' r"
-  using assms
-  unfolding crel_def by auto
+lemma crel_ifI2:
+  assumes "c \<Longrightarrow> \<exists>h' r. crel t h h' r"
+  "\<not> c \<Longrightarrow> \<exists>h' r. crel e h h' r"
+  shows "\<exists> h' r. crel (if c then t else e) h h' r"
+  oops
 
 lemma crel_option_case:
   assumes "crel (case x of None \<Rightarrow> n | Some y \<Rightarrow> s y) h h' r"
   obtains "x = None" "crel n h h' r"
         | y where "x = Some y" "crel (s y) h h' r" 
-  using assms
-  unfolding crel_def by auto
+  using assms unfolding crel_def by (auto split: option.splits)
 
 lemma crel_fold_map:
   assumes "crel (Heap_Monad.fold_map f xs) h h' r"
@@ -86,73 +43,19 @@ lemma crel_fold_map:
 using assms(1)
 proof (induct xs arbitrary: h h' r)
   case Nil  with assms(2) show ?case
-    by (auto elim: crel_return)
+    by (auto elim: crel_returnE)
 next
   case (Cons x xs)
   from Cons(2) obtain h1 y ys where crel_f: "crel (f x) h h1 y"
     and crel_fold_map: "crel (Heap_Monad.fold_map f xs) h1 h' ys"
     and r_def: "r = y#ys"
     unfolding fold_map.simps
-    by (auto elim!: crelE crel_return)
+    by (auto elim!: crel_bindE crel_returnE)
   from Cons(1)[OF crel_fold_map] crel_fold_map crel_f assms(3) r_def
   show ?case by auto
 qed
 
-
-subsection {* Elimination rules for array commands *}
-
-(* Strong version of the lemma for this operation is missing *) 
-lemma crel_new_weak:
-  assumes "crel (Array.new n v) h h' r"
-  obtains "get_array r h' = List.replicate n v"
-  using assms unfolding Array.new_def
-  by (elim crel_heap) (auto simp: array_def Let_def split_def)
-
-(* Strong version of the lemma for this operation is missing *)
-lemma crel_of_list_weak:
-  assumes "crel (Array.of_list xs) h h' r"
-  obtains "get_array r h' = xs"
-  using assms unfolding of_list_def 
-  by (elim crel_heap) (simp add: get_array_init_array_list)
-
-(* Strong version of the lemma for this operation is missing *)
-lemma crel_make_weak:
-  assumes "crel (Array.make n f) h h' r"
-  obtains "i < n \<Longrightarrow> get_array r h' ! i = f i"
-  using assms unfolding Array.make_def
-  by (elim crel_heap) (auto simp: array_def Let_def split_def)
-
-lemma crel_length:
-  assumes "crel (len a) h h' r"
-  obtains "h = h'" "r = Array.length a h'"
-  using assms unfolding Array.len_def
-  by (elim crel_tap) simp
-
-lemma crel_nth[consumes 1]:
-  assumes "crel (nth a i) h h' r"
-  obtains "r = get_array a h ! i" "h = h'" "i < Array.length a h"
-  using assms unfolding nth_def
-  by (elim crel_guard) (clarify, simp)
-
-lemma crel_upd[consumes 1]:
-  assumes "crel (upd i v a) h h' r"
-  obtains "r = a" "h' = Array.change a i v h" "i < Array.length a h"
-  using assms unfolding upd_def
-  by (elim crel_guard) simp
-
-lemma crel_map_entry:
-  assumes "crel (Array.map_entry i f a) h h' r"
-  obtains "r = a" "h' = Array.change a i (f (get_array a h ! i)) h" "i < Array.length a h"
-  using assms unfolding Array.map_entry_def
-  by (elim crel_guard) simp
-
-lemma crel_swap:
-  assumes "crel (Array.swap i x a) h h' r"
-  obtains "r = get_array a h ! i" "h' = Array.change a i x h"
-  using assms unfolding Array.swap_def
-  by (elim crel_guard) simp
-
-lemma upt_conv_Cons': (*FIXME move*)
+lemma upt_conv_Cons':
   assumes "Suc a \<le> b"
   shows "[b - Suc a..<b] = (b - Suc a)#[b - a..<b]"
 proof -
@@ -169,7 +72,7 @@ lemma crel_fold_map_nth:
 using assms
 proof (induct n arbitrary: xs h h')
   case 0 thus ?case
-    by (auto elim!: crel_return simp add: Array.length_def)
+    by (auto elim!: crel_returnE simp add: Array.length_def)
 next
   case (Suc n)
   from Suc(3) have "[Array.length a h - Suc n..<Array.length a h] = (Array.length a h - Suc n)#[Array.length a h - n..<Array.length a h]"
@@ -177,19 +80,13 @@ next
   with Suc(2) obtain r where
     crel_fold_map: "crel (Heap_Monad.fold_map (Array.nth a) [Array.length a h - n..<Array.length a h]) h h' r"
     and xs_def: "xs = get_array a h ! (Array.length a h - Suc n) # r"
-    by (auto elim!: crelE crel_nth crel_return)
+    by (auto elim!: crel_bindE crel_nthE crel_returnE)
   from Suc(3) have "Array.length a h - n = Suc (Array.length a h - Suc n)" 
     by arith
   with Suc.hyps[OF crel_fold_map] xs_def show ?case
     unfolding Array.length_def
     by (auto simp add: nth_drop')
 qed
-
-lemma crel_freeze:
-  assumes "crel (Array.freeze a) h h' xs"
-  obtains "h = h'" "xs = get_array a h"
-  using assms unfolding freeze_def
-  by (elim crel_tap) simp
 
 lemma crel_fold_map_map_entry_remains:
   assumes "crel (Heap_Monad.fold_map (\<lambda>n. map_entry n f a) [Array.length a h - n..<Array.length a h]) h h' r"
@@ -199,7 +96,7 @@ using assms
 proof (induct n arbitrary: h h' r)
   case 0
   thus ?case
-    by (auto elim: crel_return)
+    by (auto elim: crel_returnE)
 next
   case (Suc n)
   let ?h1 = "Array.change a (Array.length a h - Suc n) (f (get_array a h ! (Array.length a h - Suc n))) h"
@@ -207,7 +104,7 @@ next
     by (simp add: upt_conv_Cons')
   from Suc(2) this obtain r where
     crel_fold_map: "crel (Heap_Monad.fold_map (\<lambda>n. map_entry n f a) [Array.length a h - n..<Array.length a h]) ?h1 h' r"
-    by (auto simp add: elim!: crelE crel_map_entry crel_return)
+    by (auto simp add: elim!: crel_bindE crel_map_entryE crel_returnE)
   have length_remains: "Array.length a ?h1 = Array.length a h" by simp
   from crel_fold_map have crel_fold_map': "crel (Heap_Monad.fold_map (\<lambda>n. map_entry n f a) [Array.length a ?h1 - n..<Array.length a ?h1]) ?h1 h' r"
     by simp
@@ -224,7 +121,7 @@ using assms
 proof (induct n arbitrary: h h' r)
   case 0
   thus ?case
-    by (auto elim!: crel_return)
+    by (auto elim!: crel_returnE)
 next
   case (Suc n)
   let ?h1 = "Array.change a (Array.length a h - Suc n) (f (get_array a h ! (Array.length a h - Suc n))) h"
@@ -232,7 +129,7 @@ next
     by (simp add: upt_conv_Cons')
   from Suc(2) this obtain r where
     crel_fold_map: "crel (Heap_Monad.fold_map (\<lambda>n. map_entry n f a) [Array.length a h - n..<Array.length a h]) ?h1 h' r"
-    by (auto simp add: elim!: crelE crel_map_entry crel_return)
+    by (auto simp add: elim!: crel_bindE crel_map_entryE crel_returnE)
   have length_remains: "Array.length a ?h1 = Array.length a h" by simp
   from Suc(3) have less: "Array.length a h - Suc n < Array.length a h - n" by arith
   from Suc(3) have less2: "Array.length a h - Suc n < Array.length a h" by arith
@@ -252,7 +149,7 @@ lemma crel_fold_map_map_entry_length:
 using assms
 proof (induct n arbitrary: h h' r)
   case 0
-  thus ?case by (auto elim!: crel_return)
+  thus ?case by (auto elim!: crel_returnE)
 next
   case (Suc n)
   let ?h1 = "Array.change a (Array.length a h - Suc n) (f (get_array a h ! (Array.length a h - Suc n))) h"
@@ -260,7 +157,7 @@ next
     by (simp add: upt_conv_Cons')
   from Suc(2) this obtain r where 
     crel_fold_map: "crel (Heap_Monad.fold_map (\<lambda>n. map_entry n f a) [Array.length a h - n..<Array.length a h]) ?h1 h' r"
-    by (auto elim!: crelE crel_map_entry crel_return)
+    by (auto elim!: crel_bindE crel_map_entryE crel_returnE)
   have length_remains: "Array.length a ?h1 = Array.length a h" by simp
   from crel_fold_map have crel_fold_map': "crel (Heap_Monad.fold_map (\<lambda>n. map_entry n f a) [Array.length a ?h1 - n..<Array.length a ?h1]) ?h1 h' r"
     by simp
@@ -278,222 +175,6 @@ proof -
     by (auto intro: nth_equalityI)
 qed
 
-
-subsection {* Elimination rules for reference commands *}
-
-(* TODO:
-maybe introduce a new predicate "extends h' h x"
-which means h' extends h with a new reference x.
-Then crel_new: would be
-assumes "crel (Ref.new v) h h' x"
-obtains "get_ref x h' = v"
-and "extends h' h x"
-
-and we would need further rules for extends:
-extends h' h x \<Longrightarrow> \<not> ref_present x h
-extends h' h x \<Longrightarrow>  ref_present x h'
-extends h' h x \<Longrightarrow> ref_present y h \<Longrightarrow> ref_present y h'
-extends h' h x \<Longrightarrow> ref_present y h \<Longrightarrow> get_ref y h = get_ref y h'
-extends h' h x \<Longrightarrow> lim h' = Suc (lim h)
-*)
-
-lemma crel_ref:
-  assumes "crel (ref v) h h' x"
-  obtains "Ref.get h' x = v"
-  and "\<not> Ref.present h x"
-  and "Ref.present h' x"
-  and "\<forall>y. Ref.present h y \<longrightarrow> Ref.get h y = Ref.get h' y"
- (* and "lim h' = Suc (lim h)" *)
-  and "\<forall>y. Ref.present h y \<longrightarrow> Ref.present h' y"
-  using assms
-  unfolding Ref.ref_def
-  apply (elim crel_heap)
-  unfolding Ref.alloc_def
-  apply (simp add: Let_def)
-  unfolding Ref.present_def
-  apply auto
-  unfolding Ref.get_def Ref.set_def
-  apply auto
-  done
-
-lemma crel_lookup:
-  assumes "crel (!r') h h' r"
-  obtains "h = h'" "r = Ref.get h r'"
-  using assms unfolding Ref.lookup_def
-  by (auto elim: crel_tap)
-
-lemma crel_update:
-  assumes "crel (r' := v) h h' r"
-  obtains "h' = Ref.set r' v h" "r = ()"
-  using assms unfolding Ref.update_def
-  by (auto elim: crel_heap)
-
-lemma crel_change:
-  assumes "crel (Ref.change f r') h h' r"
-  obtains "h' = Ref.set r' (f (Ref.get h r')) h" "r = f (Ref.get h r')"
-  using assms unfolding Ref.change_def Let_def
-  by (auto elim!: crelE crel_lookup crel_update crel_return)
-
-subsection {* Elimination rules for the assert command *}
-
-lemma crel_assert[consumes 1]:
-  assumes "crel (assert P x) h h' r"
-  obtains "P x" "r = x" "h = h'"
-  using assms
-  unfolding assert_def
-  by (elim crel_if crel_return crel_raise) auto
-
-lemma crel_assert_eq: "(\<And>h h' r. crel f h h' r \<Longrightarrow> P r) \<Longrightarrow> f \<guillemotright>= assert P = f"
-unfolding crel_def bind_def Let_def assert_def
-  raise_def return_def prod_case_beta
-apply (cases f)
-apply simp
-apply (simp add: expand_fun_eq split_def)
-apply (auto split: option.split)
-apply (erule_tac x="x" in meta_allE)
-apply auto
-done
-
-section {* Introduction rules *}
-
-subsection {* Introduction rules for basic monadic commands *}
-
-lemma crelI:
-  assumes "crel f h h' r" "crel (g r) h' h'' r'"
-  shows "crel (f >>= g) h h'' r'"
-  using assms by (simp add: crel_def' bind_def)
-
-lemma crelI':
-  assumes "crel f h h' r" "crel g h' h'' r'"
-  shows "crel (f >> g) h h'' r'"
-  using assms by (intro crelI) auto
-
-lemma crel_returnI:
-  shows "crel (return x) h h x"
-  unfolding crel_def return_def by simp
-
-lemma crel_raiseI:
-  shows "\<not> (crel (raise x) h h' r)"
-  unfolding crel_def raise_def by simp
-
-lemma crel_ifI:
-  assumes "c \<longrightarrow> crel t h h' r"
-  "\<not>c \<longrightarrow> crel e h h' r"
-  shows "crel (if c then t else e) h h' r"
-  using assms
-  unfolding crel_def by auto
-
-lemma crel_option_caseI:
-  assumes "\<And>y. x = Some y \<Longrightarrow> crel (s y) h h' r"
-  assumes "x = None \<Longrightarrow> crel n h h' r"
-  shows "crel (case x of None \<Rightarrow> n | Some y \<Rightarrow> s y) h h' r"
-using assms
-by (auto split: option.split)
-
-lemma crel_tapI:
-  assumes "h' = h" "r = f h"
-  shows "crel (Heap_Monad.tap f) h h' r"
-  using assms by (simp add: crel_def)
-
-lemma crel_heapI:
-  shows "crel (Heap_Monad.heap f) h (snd (f h)) (fst (f h))"
-  by (simp add: crel_def apfst_def split_def prod_fun_def)
-
-lemma crel_heapI': (*FIXME keep only this version*)
-  assumes "h' = snd (f h)" "r = fst (f h)"
-  shows "crel (Heap_Monad.heap f) h h' r"
-  using assms
-  by (simp add: crel_def split_def apfst_def prod_fun_def)
-
-lemma crel_guardI:
-  assumes "P h" "h' = snd (f h)" "r = fst (f h)"
-  shows "crel (Heap_Monad.guard P f) h h' r"
-  using assms by (simp add: crel_def execute_simps)
-
-lemma crelI2:
-  assumes "\<exists>h' rs'. crel f h h' rs' \<and> (\<exists>h'' rs. crel (g rs') h' h'' rs)"
-  shows "\<exists>h'' rs. crel (f\<guillemotright>= g) h h'' rs"
-  oops
-
-lemma crel_ifI2:
-  assumes "c \<Longrightarrow> \<exists>h' r. crel t h h' r"
-  "\<not> c \<Longrightarrow> \<exists>h' r. crel e h h' r"
-  shows "\<exists> h' r. crel (if c then t else e) h h' r"
-  oops
-
-subsection {* Introduction rules for array commands *}
-
-lemma crel_lengthI:
-  shows "crel (Array.len a) h h (Array.length a h)"
-  unfolding len_def by (rule crel_tapI) simp_all
-
-(* thm crel_newI for Array.new is missing *)
-
-lemma crel_nthI:
-  assumes "i < Array.length a h"
-  shows "crel (nth a i) h h ((get_array a h) ! i)"
-  using assms unfolding nth_def by (auto intro: crel_guardI)
-
-lemma crel_updI:
-  assumes "i < Array.length a h"
-  shows "crel (upd i v a) h (Array.change a i v h) a"
-  using assms unfolding upd_def by (auto intro: crel_guardI)
-
-(* thm crel_of_listI is missing *)
-
-(* thm crel_map_entryI is missing *)
-
-(* thm crel_swapI is missing *)
-
-(* thm crel_makeI is missing *)
-
-(* thm crel_freezeI is missing *)
-
-(* thm crel_mapI is missing *)
-
-subsubsection {* Introduction rules for reference commands *}
-
-lemma crel_lookupI:
-  shows "crel (!r) h h (Ref.get h r)"
-  unfolding lookup_def by (auto intro!: crel_tapI)
-
-lemma crel_updateI:
-  shows "crel (r := v) h (Ref.set r v h) ()"
-  unfolding update_def by (auto intro!: crel_heapI')
-
-lemma crel_changeI: 
-  shows "crel (Ref.change f r) h (Ref.set r (f (Ref.get h r)) h) (f (Ref.get h r))"
-  unfolding change_def Let_def by (auto intro!: crelI crel_returnI crel_lookupI crel_updateI)
-
-subsubsection {* Introduction rules for the assert command *}
-
-lemma crel_assertI:
-  assumes "P x"
-  shows "crel (assert P x) h h x"
-  using assms
-  unfolding assert_def
-  by (auto intro!: crel_ifI crel_returnI crel_raiseI)
- 
-subsection {* Induction rule for the MREC combinator *}
-
-lemma MREC_induct:
-  assumes "crel (MREC f g x) h h' r"
-  assumes "\<And> x h h' r. crel (f x) h h' (Inl r) \<Longrightarrow> P x h h' r"
-  assumes "\<And> x h h1 h2 h' s z r. crel (f x) h h1 (Inr s) \<Longrightarrow> crel (MREC f g s) h1 h2 z \<Longrightarrow> P s h1 h2 z
-    \<Longrightarrow> crel (g x s z) h2 h' r \<Longrightarrow> P x h h' r"
-  shows "P x h h' r"
-proof (rule MREC_pinduct[OF assms(1)[unfolded crel_def, symmetric]])
-  fix x h h1 h2 h' s z r
-  assume "Heap_Monad.execute (f x) h = Some (Inr s, h1)"
-    "Heap_Monad.execute (MREC f g s) h1 = Some (z, h2)"
-    "P s h1 h2 z"
-    "Heap_Monad.execute (g x s z) h2 = Some (r, h')"
-  from assms(3)[unfolded crel_def, OF this(1)[symmetric] this(2)[symmetric] this(3) this(4)[symmetric]]
-  show "P x h h' r" .
-next
-qed (auto simp add: assms(2)[unfolded crel_def])
-
-
 lemma success_fold_map_map_entry:
   assumes "n \<le> Array.length a h"
   shows "success (Heap_Monad.fold_map (\<lambda>n. map_entry n f a) [Array.length a h - n..<Array.length a h]) h"
@@ -507,25 +188,26 @@ next
     (Array.length a h - Suc n) # [Array.length a h - n..<Array.length a h]"
     by (simp add: upt_conv_Cons')
   with Suc.hyps [of "(Array.change a (Array.length a h - Suc n) (f (get_array a h ! (Array.length a h - Suc n))) h)"] Suc.prems show ?case apply -
-    apply (auto simp add: execute_simps intro!: successI success_returnI success_map_entryI elim: crel_map_entry)
-    apply (subst execute_bind) apply (auto simp add: execute_simps)
+    apply (auto simp add: execute_simps execute_bind_success intro!: successI success_returnI success_map_entryI elim: crel_map_entryE)
+    apply (subst execute_bind) apply (auto simp add: execute_simps execute_bind_success intro: execute_bind)
     done
 qed
 
-
-section {* Cumulative lemmas *}
-
-lemmas crel_elim_all =
-  crelE crelE' crel_return crel_raise crel_if crel_option_case
-  crel_length crel_new_weak crel_nth crel_upd crel_of_list_weak crel_map_entry crel_swap crel_make_weak crel_freeze
-  crel_ref crel_lookup crel_update crel_change
-  crel_assert
-
-lemmas crel_intro_all =
-  crelI crelI' crel_returnI crel_raiseI crel_ifI crel_option_caseI
-  crel_lengthI (* crel_newI *) crel_nthI crel_updI (* crel_of_listI crel_map_entryI crel_swapI crel_makeI crel_freezeI crel_mapI *)
-  (* crel_Ref_newI *) crel_lookupI crel_updateI crel_changeI
-  crel_assert
-
+lemma MREC_induct:
+  assumes "crel (MREC f g x) h h' r"
+  assumes "\<And> x h h' r. crel (f x) h h' (Inl r) \<Longrightarrow> P x h h' r"
+  assumes "\<And> x h h1 h2 h' s z r. crel (f x) h h1 (Inr s) \<Longrightarrow> crel (MREC f g s) h1 h2 z \<Longrightarrow> P s h1 h2 z
+    \<Longrightarrow> crel (g x s z) h2 h' r \<Longrightarrow> P x h h' r"
+  shows "P x h h' r"
+proof (rule MREC_pinduct[OF assms(1) [unfolded crel_def]])
+  fix x h h1 h2 h' s z r
+  assume "Heap_Monad.execute (f x) h = Some (Inr s, h1)"
+    "Heap_Monad.execute (MREC f g s) h1 = Some (z, h2)"
+    "P s h1 h2 z"
+    "Heap_Monad.execute (g x s z) h2 = Some (r, h')"
+  from assms(3) [unfolded crel_def, OF this(1) this(2) this(3) this(4)]
+  show "P x h h' r" .
+next
+qed (auto simp add: assms(2)[unfolded crel_def])
 
 end
