src/HOL/Imperative_HOL/Imperative_HOL_ex.thy
@@ -6,8 +6,8 @@
 header {* Monadic imperative HOL with examples *}
 
 theory Imperative_HOL_ex
-imports Imperative_HOL "ex/Imperative_Quicksort" "ex/Imperative_Reverse" "ex/Linked_Lists"
-  "ex/SatChecker"
+imports Imperative_HOL
+  "ex/Imperative_Quicksort" "ex/Imperative_Reverse" "ex/Linked_Lists" "ex/SatChecker"
 begin
 
 end
