src/HOL/Imperative_HOL/ex/Linked_Lists.thy
@@ -5,7 +5,7 @@
 header {* Linked Lists by ML references *}
 
 theory Linked_Lists
-imports "~~/src/HOL/Imperative_HOL/Imperative_HOL" Code_Integer
+imports Imperative_HOL Code_Integer
 begin
 
 section {* Definition of Linked Lists *}
@@ -42,7 +42,7 @@ text {* define traverse using the MREC combinator *}
 definition
   traverse :: "'a\<Colon>heap node \<Rightarrow> 'a list Heap"
 where
-  "traverse = MREC (\<lambda>n. case n of Empty \<Rightarrow> return (Inl [])
+[code del]: "traverse = MREC (\<lambda>n. case n of Empty \<Rightarrow> return (Inl [])
                                 | Node x r \<Rightarrow> (do tl \<leftarrow> Ref.lookup r;
                                                   return (Inr tl) done))
                    (\<lambda>n tl xs. case n of Empty \<Rightarrow> undefined
@@ -452,18 +452,37 @@ next
     by simp
 qed
 
+lemma crel_ref:
+  assumes "crel (ref v) h h' x"
+  obtains "Ref.get h' x = v"
+  and "\<not> Ref.present h x"
+  and "Ref.present h' x"
+  and "\<forall>y. Ref.present h y \<longrightarrow> Ref.get h y = Ref.get h' y"
+ (* and "lim h' = Suc (lim h)" *)
+  and "\<forall>y. Ref.present h y \<longrightarrow> Ref.present h' y"
+  using assms
+  unfolding Ref.ref_def
+  apply (elim crel_heapE)
+  unfolding Ref.alloc_def
+  apply (simp add: Let_def)
+  unfolding Ref.present_def
+  apply auto
+  unfolding Ref.get_def Ref.set_def
+  apply auto
+  done
+
 lemma make_llist:
 assumes "crel (make_llist xs) h h' r"
 shows "list_of h' r xs \<and> (\<forall>rs. refs_of h' r rs \<longrightarrow> (\<forall>ref \<in> (set rs). Ref.present h' ref))"
 using assms 
 proof (induct xs arbitrary: h h' r)
-  case Nil thus ?case by (auto elim: crel_return simp add: make_llist.simps)
+  case Nil thus ?case by (auto elim: crel_returnE simp add: make_llist.simps)
 next
   case (Cons x xs')
   from Cons.prems obtain h1 r1 r' where make_llist: "crel (make_llist xs') h h1 r1"
     and crel_refnew:"crel (ref r1) h1 h' r'" and Node: "r = Node x r'"
     unfolding make_llist.simps
-    by (auto elim!: crelE crel_return)
+    by (auto elim!: crel_bindE crel_returnE)
   from Cons.hyps[OF make_llist] have list_of_h1: "list_of h1 r1 xs'" ..
   from Cons.hyps[OF make_llist] obtain rs' where rs'_def: "refs_of h1 r1 rs'" by (auto intro: list_of_refs_of)
   from Cons.hyps[OF make_llist] rs'_def have refs_present: "\<forall>ref\<in>set rs'. Ref.present h1 ref" by simp
@@ -472,11 +491,11 @@ next
     by (auto elim!: crel_ref dest: refs_of_is_fun)
   with list_of_invariant[OF list_of_h1 refs_unchanged] Node crel_refnew have fstgoal: "list_of h' r (x # xs')"
     unfolding list_of.simps
-    by (auto elim!: crel_ref)
+    by (auto elim!: crel_refE)
   from refs_unchanged rs'_def have refs_still_present: "\<forall>ref\<in>set rs'. Ref.present h' ref" by auto
   from refs_of_invariant[OF rs'_def refs_unchanged] refs_unchanged Node crel_refnew refs_still_present
   have sndgoal: "\<forall>rs. refs_of h' r rs \<longrightarrow> (\<forall>ref\<in>set rs. Ref.present h' ref)"
-    by (fastsimp elim!: crel_ref dest: refs_of_is_fun)
+    by (fastsimp elim!: crel_refE dest: refs_of_is_fun)
   from fstgoal sndgoal show ?case ..
 qed
 
@@ -489,7 +508,7 @@ next
   case (Cons x xs)
   thus ?case
   apply (cases n, auto)
-  by (auto intro!: crelI crel_returnI crel_lookupI)
+  by (auto intro!: crel_bindI crel_returnI crel_lookupI)
 qed
 
 lemma traverse_make_llist':
@@ -499,7 +518,7 @@ proof -
   from crel obtain h1 r1
     where makell: "crel (make_llist xs) h h1 r1"
     and trav: "crel (traverse r1) h1 h' r"
-    by (auto elim!: crelE)
+    by (auto elim!: crel_bindE)
   from make_llist[OF makell] have "list_of h1 r1 xs" ..
   from traverse [OF this] trav show ?thesis
     using crel_deterministic by fastsimp
@@ -551,7 +570,7 @@ proof (induct ps arbitrary: qs p q h)
   case Nil
   thus ?case
     unfolding rev'_simps[of q p] list_of'_def
-    by (auto elim!: crelE crel_lookup crel_return)
+    by (auto elim!: crel_bindE crel_lookupE crel_returnE)
 next
   case (Cons x xs)
   (*"LinkedList.list_of h' (get_ref v h') (List.rev xs @ x # qsa)"*)
@@ -561,7 +580,7 @@ next
     and list_of'_ref: "list_of' h ref xs"
     unfolding list_of'_def by (cases "Ref.get h p", auto)
   from p_is_Node Cons(2) have crel_rev': "crel (rev' (p, ref)) (Ref.set p (Node x q) h) h' v"
-    by (auto simp add: rev'_simps [of q p] elim!: crelE crel_lookup crel_update)
+    by (auto simp add: rev'_simps [of q p] elim!: crel_bindE crel_lookupE crel_updateE)
   from Cons(3) obtain qrs where qrs_def: "refs_of' h q qrs" by (elim list_of'_refs_of')
   from Cons(4) obtain prs where prs_def: "refs_of' h p prs" by (elim list_of'_refs_of')
   from qrs_def prs_def Cons(5) have distinct_pointers: "set qrs \<inter> set prs = {}" by fastsimp
@@ -602,7 +621,7 @@ using assms
 proof (cases r)
   case Empty
   with list_of_h crel_rev show ?thesis
-    by (auto simp add: list_of_Empty elim!: crel_return)
+    by (auto simp add: list_of_Empty elim!: crel_returnE)
 next
   case (Node x ps)
   with crel_rev obtain p q h1 h2 h3 v where
@@ -611,7 +630,7 @@ next
     and crel_rev':"crel (rev' (q, p)) h2 h3 v"
     and lookup: "crel (!v) h3 h' r'"
     using rev.simps
-    by (auto elim!: crelE)
+    by (auto elim!: crel_bindE)
   from init have a1:"list_of' h2 q []"
     unfolding list_of'_def
     by (auto elim!: crel_ref)
@@ -622,7 +641,7 @@ next
   from init this Node have a2: "list_of' h2 p xs"
     apply -
     unfolding list_of'_def
-    apply (auto elim!: crel_ref)
+    apply (auto elim!: crel_refE)
     done
   from init have refs_of_q: "refs_of' h2 q [q]"
     by (auto elim!: crel_ref)
@@ -633,15 +652,15 @@ next
     by (fastsimp elim!: crel_ref dest: refs_of'_is_fun)
   from refs_of'_invariant[OF refs_of'_ps this] have "refs_of' h2 ps refs" .
   with init have refs_of_p: "refs_of' h2 p (p#refs)"
-    by (auto elim!: crel_ref simp add: refs_of'_def')
+    by (auto elim!: crel_refE simp add: refs_of'_def')
   with init all_ref_present have q_is_new: "q \<notin> set (p#refs)"
-    by (auto elim!: crel_ref intro!: Ref.noteq_I)
+    by (auto elim!: crel_refE intro!: Ref.noteq_I)
   from refs_of_p refs_of_q q_is_new have a3: "\<forall>qrs prs. refs_of' h2 q qrs \<and> refs_of' h2 p prs \<longrightarrow> set prs \<inter> set qrs = {}"
     by (fastsimp simp only: set.simps dest: refs_of'_is_fun)
   from rev'_invariant [OF crel_rev' a1 a2 a3] have "list_of h3 (Ref.get h3 v) (List.rev xs)" 
     unfolding list_of'_def by auto
   with lookup show ?thesis
-    by (auto elim: crel_lookup)
+    by (auto elim: crel_lookupE)
 qed
 
 
@@ -796,13 +815,13 @@ proof (induct arbitrary: h' r rule: merge_induct2[OF assms(1) assms(2)])
   case (1 ys p q)
   from 1(3-4) have "h = h' \<and> r = q"
     unfolding merge_simps[of p q]
-    by (auto elim!: crel_lookup crelE crel_return)
+    by (auto elim!: crel_lookupE crel_bindE crel_returnE)
   with assms(4)[OF 1(1) 1(2) 1(3)] show ?case by simp
 next
   case (2 x xs' p q pn)
   from 2(3-5) have "h = h' \<and> r = p"
     unfolding merge_simps[of p q]
-    by (auto elim!: crel_lookup crelE crel_return)
+    by (auto elim!: crel_lookupE crel_bindE crel_returnE)
   with assms(5)[OF 2(1-4)] show ?case by simp
 next
   case (3 x xs' y ys' p q pn qn)
@@ -810,7 +829,7 @@ next
     1: "crel (merge pn q) h h1 r1" 
     and 2: "h' = Ref.set p (Node x r1) h1 \<and> r = p"
     unfolding merge_simps[of p q]
-    by (auto elim!: crel_lookup crelE crel_return crel_if crel_update)
+    by (auto elim!: crel_lookupE crel_bindE crel_returnE crel_ifE crel_updateE)
   from 3(6)[OF 1] assms(6) [OF 3(1-5)] 1 2 show ?case by simp
 next
   case (4 x xs' y ys' p q pn qn)
@@ -818,7 +837,7 @@ next
     1: "crel (merge p qn) h h1 r1" 
     and 2: "h' = Ref.set q (Node y r1) h1 \<and> r = q"
     unfolding merge_simps[of p q]
-    by (auto elim!: crel_lookup crelE crel_return crel_if crel_update)
+    by (auto elim!: crel_lookupE crel_bindE crel_returnE crel_ifE crel_updateE)
   from 4(6)[OF 1] assms(7) [OF 4(1-5)] 1 2 show ?case by simp
 qed
 
